Ajout balisage

src/CoqNom/examples/example3Raff.v
@@ -6,29 +6,35 @@ From FreeMonad Require Import FreeMonad.
 
 Section PHOAS.
 
-  Context {var : Type -> Type}.
+(* =var= *)
+Context {var : Type -> Type}.
+(* =end= *)
 
-  Inductive VAL : Type -> Type :=
-  | Var : forall {X}, var X -> VAL X
-  | Const : N -> VAL N
-  | Add : VAL N -> VAL N -> VAL N
-  | Sub : VAL N -> VAL N -> VAL N
-  | Le : VAL N -> VAL N -> VAL bool
-  | Lt : VAL N -> VAL N -> VAL bool
-  | Len : VAL span -> VAL N
-  | Pair : forall {X Y}, VAL X -> VAL Y -> VAL (X * Y)
-  | Fst : forall {X Y}, VAL (X * Y) -> VAL X
-  | Snd : forall {X Y}, VAL (X * Y) -> VAL Y
-  | ToU32 : VAL octet -> VAL octet -> VAL octet -> VAL octet -> VAL N.
+(* =VAL= *)
+Inductive VAL : Type -> Type :=
+| Var : forall {X}, var X -> VAL X
+| Const : N -> VAL N
+| Add : VAL N -> VAL N -> VAL N
+| Sub : VAL N -> VAL N -> VAL N
+| Le : VAL N -> VAL N -> VAL bool
+| Lt : VAL N -> VAL N -> VAL bool
+| Len : VAL span -> VAL N
+| Pair : forall {X Y}, VAL X -> VAL Y -> VAL (X * Y)
+| Fst : forall {X Y}, VAL (X * Y) -> VAL X
+| Snd : forall {X Y}, VAL (X * Y) -> VAL Y
+| ToU32 : VAL octet -> VAL octet -> VAL octet -> VAL octet -> VAL N.
+(* =end= *)
 
-  Inductive Expr : Type -> Type :=
-  | Val : forall {X}, VAL X -> Expr X
-  | LetIn : forall {X}, Expr X -> forall {Y}, (var X -> Expr Y) -> Expr Y
-  | IfThenElse: VAL bool -> forall {X}, Expr X -> Expr X -> Expr X
-  | Take : VAL N -> Expr span
-  | Read : VAL span -> VAL N -> Expr octet
-  | Length : Expr N
-  | Fail : forall {X}, Expr X.
+(* =Expr= *)
+Inductive Expr : Type -> Type :=
+| Val : forall {X}, VAL X -> Expr X
+| LetIn : forall {X}, Expr X -> forall {Y}, (var X -> Expr Y) -> Expr Y
+| IfThenElse: VAL bool -> forall {X}, Expr X -> Expr X -> Expr X
+| Take : VAL N -> Expr span
+| Read : VAL span -> VAL N -> Expr octet
+| Length : Expr N
+| Fail : forall {X}, Expr X.
+(* =end= *)
 
 End PHOAS.
 
@@ -42,95 +48,100 @@ Notation "'(!' a ',' b ')'" := (Pair a b)(at level 25, left associativity).
 
 Section sem_PHOAS.
 
+(* =ID= *)
+Definition ID (X : Type) := X.
+(* =end= *)
 
-  Inductive var : Type -> Type :=
-  | VNat : N -> var N
-  | VSpan : span -> var span
-  | VBool : bool -> var bool
-  | VPair : forall {X Y}, var X -> var Y -> var (X * Y).
-
-  Fixpoint sem_val {X} (v : var X) : X :=
-  match v with
-  | VSpan v | VBool v | VNat v => v
-  | VPair va vb => (sem_val va, sem_val vb)
+Definition lookup_default (data : data) n default :=
+  match lookup n data with
+  | Some v => v
+  | None => default
   end.
 
-  Inductive sem_VAL : forall {X}, @VAL var X -> var X -> Prop :=
-  | sem_Const : forall n, sem_VAL (Const n) (VNat n)
-  | sem_Add : forall vm m m' vn n n',
-      sem_val m = m' ->
-      sem_VAL vm m ->
-      sem_val n = n' ->
-      sem_VAL vn n ->
-      sem_VAL (Add vm vn) (VNat (m' + n'))
-  | sem_Sub : forall vm m m' vn n n',
-      sem_val m = m' ->
-      sem_VAL vm m ->
-      sem_val n = n' ->
-      sem_VAL vn n ->
-      sem_VAL (Sub vm vn) (VNat (m' - n'))
-  | sem_Le : forall vm vn m m' n n',
-      sem_VAL vm m ->
-      sem_val m = m' ->
-      sem_VAL vn n ->
-      sem_val n = n' ->
-      sem_VAL (Le vm vn) (VBool (m' <=? n'))
-  | sem_Lt : forall vm vn m n,
-      sem_VAL vm m ->
-      sem_VAL vn n ->
-      sem_VAL (Lt vm vn) (VBool (sem_val m <? sem_val n))
-  | sem_Len : forall vs s,
-      sem_VAL vs s ->
-      sem_VAL (Len vs) (VNat (len (sem_val s)))
-  | sem_Pair : forall X Y va (a : var X) vb (b : var Y),
-      sem_VAL va a ->
-      sem_VAL vb b ->
-      sem_VAL (Pair va vb) (VPair a b)
-  | sem_Fst : forall X Y v (a : var X) (b : var Y),
-      sem_VAL v (VPair a b) ->
-      sem_VAL (Fst v) a
-  | sem_Snd : forall X Y v (a : var X) (b : var Y),
-      sem_VAL v (VPair a b) ->
-      sem_VAL (Snd v) b
-  | sem_ToU32 : forall va vb vc vd a b c d,
-      sem_VAL va a ->
-      sem_VAL vb b ->
-      sem_VAL vc c ->
-      sem_VAL vd d ->
-      sem_VAL (ToU32 va vb vc vd) (VNat (to_u32 (sem_val a) (sem_val b) (sem_val c) (sem_val d)))
-  | sem_Var : forall X (v : var X), sem_VAL (Var v) v.
+(* =sem_VAL= *)
+Inductive sem_VAL : forall {X}, @VAL ID X -> ID X -> Prop :=
+(* =end= *)
+| sem_Const : forall n, sem_VAL (Const n) n
+(* =sem_Add= *)
+| sem_Add : forall vm m vn n,
+    sem_VAL vm m ->
+    sem_VAL vn n ->
+    sem_VAL (Add vm vn) (m + n)
+(* =end= *)
+| sem_Sub : forall vm m vn n,
+    sem_VAL vm m ->
+    sem_VAL vn n ->
+    sem_VAL (Sub vm vn) (m - n)
+| sem_Le : forall vm vn m n,
+    sem_VAL vm m ->
+    sem_VAL vn n ->
+    sem_VAL (Le vm vn) (m <=? n)
+| sem_Lt : forall vm vn m n,
+    sem_VAL vm m ->
+    sem_VAL vn n ->
+    sem_VAL (Lt vm vn) (m <? n)
+| sem_Len : forall vs s,
+    sem_VAL vs s ->
+    sem_VAL (Len vs) (len s)
+| sem_Pair : forall X Y va (a : ID X) vb (b : ID Y),
+    sem_VAL va a ->
+    sem_VAL vb b ->
+    sem_VAL (Pair va vb) (a,b)
+| sem_Fst : forall X Y v (a : ID X) (b : ID Y),
+    sem_VAL v (a, b) ->
+    sem_VAL (Fst v) a
+| sem_Snd : forall X Y v (a : ID X) (b : ID Y),
+    sem_VAL v (a, b) ->
+    sem_VAL (Snd v) b
+| sem_ToU32 : forall va vb vc vd a b c d,
+    sem_VAL va a ->
+    sem_VAL vb b ->
+    sem_VAL vc c ->
+    sem_VAL vd d ->
+    sem_VAL (ToU32 va vb vc vd) (to_u32 a b c d)
+| sem_Var : forall X (v : ID X), sem_VAL (Var v) v.
 
+(* =sem_Expr= *)
+Inductive sem_Expr {data : list N} :
+  span -> forall {X}, @Expr ID X -> option (ID X * span) -> Prop
+(* =end= *)
+:=
+| sem_Val : forall s X (v :VAL X) res,
+    sem_VAL v res ->
+    sem_Expr s (Val v) (Some (res, s))
+| sem_LetInF : forall X ex Y (k : X -> Expr Y) s,
+    sem_Expr s ex None ->
+    sem_Expr s (LetIn ex k) None
+| sem_LetInS : forall X ex Y (k : X -> Expr Y) s v sv res,
+    sem_Expr s ex (Some (v, sv)) ->
+    sem_Expr sv (k v) res ->
+    sem_Expr s (LetIn ex k) res
+| sem_IfThenElseT : forall vb X (et ee : Expr X) res s,
+    sem_VAL vb true ->
+    sem_Expr s et res ->
+    sem_Expr s (IfThenElse vb et ee) res
+| sem_IfThenElseF : forall vb X (et ee : Expr X) res s,
+    sem_VAL vb false ->
+    sem_Expr s ee res ->
+    sem_Expr s (IfThenElse vb et ee) res
 
-  Inductive sem_Expr {data : list N} :
-    span -> forall {X}, @Expr var X -> option (var X * span) -> Prop :=
-  | sem_Val : forall s X (v :VAL X) res,
-      sem_VAL v res ->
-      sem_Expr s (Val v) (Some (res, s))
-  | sem_LetInF : forall X ex Y (k : var X -> Expr Y) s,
-      sem_Expr s ex None ->
-      sem_Expr s (LetIn ex k) None
-  | sem_LetInS : forall X ex Y (k : var X -> Expr Y) s v sv res,
-      sem_Expr s ex (Some (v, sv)) ->
-      sem_Expr sv (k v) res ->
-      sem_Expr s (LetIn ex k) res
-  | sem_IfThenElseT : forall vb X (et ee : Expr X) res s,
-      sem_VAL vb (VBool true) ->
-      sem_Expr s et res ->
-      sem_Expr s (IfThenElse vb et ee) res
-  | sem_IfThenElseF : forall vb X (et ee : Expr X) res s,
-      sem_VAL vb (VBool false) ->
-      sem_Expr s ee res ->
-      sem_Expr s (IfThenElse vb et ee) res
-  | sem_Take : forall s vn n,
-    sem_VAL vn (VNat n) ->
-    sem_Expr s (Take vn) (Some (VSpan (mk_span (pos s) n), mk_span (pos s + n) (len s - n)))
-  | sem_Read : forall s vrange range vn n v default,
-      sem_VAL vrange (VSpan range) ->
-      sem_VAL vn (VNat n) ->
-      nth (N.to_nat (pos range + n)) data default = v ->
-      sem_Expr s (Read vrange vn) (Some (VNat v, s))
-  | sem_Length : forall s, sem_Expr s Length (Some (VNat (len s), s))
-  | sem_Fail : forall X s, sem_Expr s (Fail : Expr X) None.
+(* =sem_Take= *)
+| sem_Take : forall s vn n,
+    sem_VAL vn n ->
+    sem_Expr s (Take vn) (Some ({| pos := pos s; len := n |},
+                                {| pos := pos s + n; len := len s - n |}))
+(* =end= *)
+
+(* =sem_Read= *)
+| sem_Read : forall s vrange range vn n v default,
+    sem_VAL vrange range ->
+    sem_VAL vn n ->
+    lookup_default data (pos range + n) default = v ->
+    sem_Expr s (Read vrange vn) (Some (v, s))
+(* =end= *)
+
+| sem_Length : forall s, sem_Expr s Length (Some (len s, s))
+| sem_Fail : forall X s, sem_Expr s (Fail : Expr X) None.
 
 End sem_PHOAS.
 
@@ -144,7 +155,7 @@ Definition adequate {X Y} (R : X -> Y -> Prop) (d : Decodeur X) (e : Expr Y) (da
     @sem_Expr data s Y e res ->
     match res with
     | None => eval d data s = None
-    | Some (v, t) => ∃ r, eval d data s = Some (r, t) /\ R r (sem_val v)
+    | Some (v, t) => ∃ r, eval d data s = Some (r, t) /\ R r v
     end.
 
 Axiom adequacy_pure : forall X e (Q : X -> Prop),
@@ -161,7 +172,7 @@ Lemma adequacy_pure_PHOAS :
       forall vv s sres,
         @sem_Expr data s X h (Some (vv, sres)) ->
         span_data_wf data s ->
-        Q (sem_val vv).
+        Q vv.
 Proof.
   intros X Q e h TRIPLE data ADE vv s sres SEM WF.
   eapply ADE in SEM as [r [EVAL EQ]]; eauto. subst.
@@ -208,15 +219,15 @@ Ltac sem_VAL_unif :=
   | H : sem_VAL ?t _, H0 : sem_VAL ?t _ |- _ => eapply (sem_VAL_inj _ t _ _ H) in H0
   end.
 
-Ltac inj_val :=
-  match goal with
-  | H : VNat _ = VNat _ |- _ => injection H; intros; clear H
-  | H : VSpan _ = VSpan _ |- _ => injection H; intros; clear H
-  | H : VBool _ = VBool _ |- _ => injection H; intros; clear H
-  | H : VPair _ _ = VPair _ _ |- _ => injection H; intros; clear H
-  end.
+(* Ltac inj_val := *)
+(*   match goal with *)
+(*   | H : VNat _ = VNat _ |- _ => injection H; intros; clear H *)
+(*   | H : VSpan _ = VSpan _ |- _ => injection H; intros; clear H *)
+(*   | H : VBool _ = VBool _ |- _ => injection H; intros; clear H *)
+(*   | H : VPair _ _ = VPair _ _ |- _ => injection H; intros; clear H *)
+(*   end. *)
 
-Ltac VAL_unif := repeat sem_VAL_unif; repeat inj_val.
+Ltac VAL_unif := repeat sem_VAL_unif.
 
 Open Scope free_monad_scope.
 
@@ -226,9 +237,9 @@ Axiom run_bind_fail : forall s data X Y e (k : X -> Decodeur Y),
 
 Lemma bind_adequate :
   forall data (X X0 Y Y0 : Type) R R0 (e : Decodeur X) (ke : X -> Decodeur Y)
-    (h : Expr X0) (kh : var X0 -> Expr Y0),
+    (h : Expr X0) (kh : X0 -> Expr Y0),
     adequate R0 e h data ->
-    (forall res vres, R0 res (sem_val vres) -> adequate R (ke res) (kh vres) data) ->
+    (forall res vres, R0 res vres -> adequate R (ke res) (kh vres) data) ->
     adequate R (let! v := e in ke v) (let% v := h in kh v) data.
 Proof.
   unfold adequate.
@@ -249,7 +260,7 @@ Admitted.
 Lemma ret_adequate :
   forall Y (va : VAL Y) (X : Type) (R : X -> Y -> Prop) a (v : X) data,
     sem_VAL va a ->
-    R v (sem_val a) ->
+    R v a ->
     adequate R (ret v) (Val va) data.
 Proof.
   unfold adequate.
@@ -260,26 +271,25 @@ Qed.
 Definition span_eq_take data n (s0 s1 : span) : Prop :=
   s0 = s1 /\ span_data_wf data s1 /\ len s1 = n.
 
-Lemma take_adequate : forall (hn : VAL N) data (n : N) vn,
-    sem_VAL hn vn ->
-    sem_val vn = n ->
+Lemma take_adequate : forall (hn : VAL N) data (n : N),
+    sem_VAL hn n ->
     adequate (span_eq_take data n) (take n)
       (let% len := Length in
        IfThenElse (Le hn (Var len))
          (Take hn)
          Fail) data.
 Proof.
-  intros data n hn vn VALN EQ s res WF SEM.
+  intros hn data n VALN s res WF SEM.
   next_step SEM.
   - next_step H2.
   - next_step H6.
-    + next_step H3. next_step H8. next_step H4. next_step H6.
+    + next_step H3. next_step H8. next_step H4. next_step H5.
       simpl in *. repeat VAL_unif. subst.
       simpl. unfold example2.bind. unfold takeM.
       eexists. rewrite H1. split. reflexivity.
       repeat split. unfold span_data_wf in *. simpl.
       eapply N.leb_le in H1. simpl in *. lia.
-    + next_step H8. next_step H4. next_step H3. next_step H6.
+    + next_step H8. next_step H4. next_step H5. next_step H3.
       repeat VAL_unif. subst.
       simpl. unfold example2.bind. unfold takeM.
       rewrite H1. reflexivity.
@@ -305,7 +315,7 @@ Qed.
 
 Lemma lookup_nth : forall pos (data : data) default,
     pos < length data ->
-    lookup pos data = Some (nth (N.to_nat pos) data default).
+    lookup pos data = Some (lookup_default data pos default).
 Proof.
   induction pos using N.peano_ind; simpl; intros data default LT.
   - destruct data; simpl in *; intros.
@@ -316,37 +326,38 @@ Proof.
     + rewrite length_equation_2 in LT. eapply N.succ_lt_mono in LT.
       eapply IHpos in LT. rewrite <- N.succ_pos_spec.
       rewrite lookup_equation_3. rewrite N.succ_pos_spec. rewrite N.pred_succ.
-      erewrite LT. f_equal. rewrite N2Nat.inj_succ. reflexivity.
+      erewrite LT.
+      f_equal. unfold lookup_default. rewrite <- N.succ_pos_spec.
+      rewrite lookup_equation_3. rewrite N.succ_pos_spec. rewrite N.pred_succ.
+      reflexivity.
 Qed.
 
-Lemma read_adequate : forall hs hn data vn (n n0 : N) vs s,
-    span_eq_take data n0 s (sem_val vs) ->
-    sem_VAL hs vs ->
-    sem_VAL hn vn ->
-    sem_val vn = n ->
+Lemma read_adequate : forall hs hn data (n n0 : N) s,
+    span_eq_take data n0 s s ->
+    sem_VAL hs s ->
+    sem_VAL hn n ->
     adequate eq (read s n) (IfThenElse (Lt hn (Len hs)) (Read hs hn) Fail) data.
 Proof.
-  intros hs hn data vn n n0 vs s RS ADES ADEN VALn s0 res WF SEM.
+  intros hs hn data n n0 s RS ADES ADEN s0 res WF SEM.
   next_step SEM.
   - next_step H3. next_step H4. next_step H6. repeat VAL_unif. subst. simpl in *.
     destruct RS as [P0 [P1 P2]]. subst.
     unfold example2.bind, readM. rewrite H1. eapply N.ltb_lt in H1.
-    rewrite (lookup_nth (pos range + n) data default).
+    rewrite (lookup_nth (pos range + n1) data default).
     eexists. split; auto. unfold span_data_wf in P1. lia.
   - next_step H6. next_step H3. next_step H4. repeat VAL_unif. subst. simpl in *.
     destruct RS as [P0 [P1 P2]]. subst.
     unfold example2.bind, readM. rewrite H1. reflexivity.
 Qed.
 
-Lemma read2_adequate : forall hs hn data vn (n n0 : N) vs s,
-    span_eq_take data n0 s (sem_val vs) ->
-    sem_VAL hs vs ->
-    sem_VAL hn vn ->
-    sem_val vn = n ->
+Lemma read2_adequate : forall hs hn data (n n0 : N) s,
+    span_eq_take data n0 s s ->
+    sem_VAL hs s ->
+    sem_VAL hn n ->
     n < n0 ->
     adequate eq (read s n) (Read hs hn) data.
 Proof.
-  intros hs hn data vn n n0 vs s RS ADES ADEN VALn LT s0 res WF SEM.
+  intros hs hn data n n0 s RS ADES ADEN LT s0 res WF SEM.
   next_step SEM.
   repeat VAL_unif. subst. simpl. unfold example2.bind, readM. eapply N.ltb_lt in LT.
   destruct RS as [P0 [P1 P2]]. subst.
@@ -355,14 +366,13 @@ Proof.
   eexists. split; auto. lia.
 Qed.
 
-Lemma ite_adequate : forall hb data X Y R vb (b : bool) (et : Decodeur X) (ht : Expr Y) ef hf,
-    sem_VAL hb vb ->
-    sem_val vb = b ->
+Lemma ite_adequate : forall hb data X Y R (b : bool) (et : Decodeur X) (ht : Expr Y) ef hf,
+    sem_VAL hb b ->
     (b = true -> adequate R et ht data) ->
     (b = false -> adequate R ef hf data) ->
     adequate R (if b then et else ef) (IfThenElse hb ht hf) data.
 Proof.
-  intros hb data X Y R vb b et ht ef hf VALb EQ ADET ADEF s res WF SEM.
+  intros hb data X Y R b et ht ef hf EQ ADET ADEF s res WF SEM.
   subst. next_step SEM.
   - repeat VAL_unif. subst. simpl. eapply ADET; auto.
   - repeat VAL_unif. subst. simpl. eapply ADEF; auto.
@@ -387,20 +397,25 @@ Ltac N_is_literal n :=
 
 Ltac what_is e k :=
   match e with
-  | ?e => N_is_literal e; k (@Const var e)
-  (* | H : ?e = sem_val ?v |- ?e => is_var e; k (@Var var v) *)
+  | ?e => N_is_literal e; k (@Const ID e)
+  | _ =>
+      match goal with
+      | H : sem_VAL ?v e |- _ => k v
+      | H : ?v = e |- _ => is_var e; k (@Var ID v)
+      | H : e = ?v |- _ => is_var e; k (@Var ID v)
+      end
   (* | H : sem_val ?v = ?e |- ?e => is_var e; k (@Var var v) *)
   (* | ?e => is_var e; k (@Var _ var e) *)
-  | sem_val ?e => is_var e; k (@Var var _ e)
-  | ?l <=? ?r => what_is l ltac:(fun l => what_is r ltac:(fun r => k (@Le var l r)))
-  | ?l <? ?r => what_is l ltac:(fun l => what_is r ltac:(fun r => k (@Lt var l r)))
-  | ?l + ?r => what_is l ltac:(fun l => what_is r ltac:(fun r => k (@Add var l r)))
-  | ?l - ?r => what_is l ltac:(fun l => what_is r ltac:(fun r => k (@Sub var l r)))
+  | ?l <=? ?r => what_is l ltac:(fun l => what_is r ltac:(fun r => k (@Le ID l r)))
+  | ?l <? ?r => what_is l ltac:(fun l => what_is r ltac:(fun r => k (@Lt ID l r)))
+  | ?l + ?r => what_is l ltac:(fun l => what_is r ltac:(fun r => k (@Add ID l r)))
+  | ?l - ?r => what_is l ltac:(fun l => what_is r ltac:(fun r => k (@Sub ID l r)))
   | to_u32 ?a ?b ?c ?d =>
       what_is a ltac:(fun a =>
        what_is b ltac:(fun b =>
         what_is c ltac:(fun c =>
-         what_is d ltac:(fun d => k (@ToU32 var a b c d)))))
+                          what_is d ltac:(fun d => k (@ToU32 ID a b c d)))))
+  | ?e => is_var e; k (@Var ID _ e)
   end.
 
 Ltac clean_up :=
@@ -415,15 +430,15 @@ Ltac clean_up :=
 Ltac step := repeat clean_up; subst;
   match goal with
   | |- adequate _ (let! _ := _ in _) _ _ =>
-        eapply bind_adequate; [ idtac | intros (* intros; repeat clean_up; subst *) ]
+        eapply bind_adequate; [ idtac | intros  ]
   | |- adequate _ (take ?e) _ _ =>
       what_is e ltac:(fun v => eapply (take_adequate v)); repeat econstructor
   | |- adequate _ (read ?s ?n) _ _ =>
       what_is s ltac:(fun s => what_is n ltac:(fun n => eapply (read2_adequate s n)));
-      [repeat split; eauto | repeat econstructor | repeat econstructor | eauto | lia]
+      [repeat split; eauto | repeat econstructor | repeat econstructor | lia]
   | |- adequate _ (read ?s ?n) _ _ =>
       what_is s ltac:(fun s => what_is n ltac:(fun n => eapply (read_adequate s n)));
-      [repeat split; eauto | repeat econstructor | repeat econstructor | eauto]
+      [repeat split; eauto | repeat econstructor | repeat econstructor]
   | |- adequate _ (if ?b then ?et else ?ef) _ _ =>
       what_is b ltac:(fun s => eapply (ite_adequate s));
       repeat econstructor; eauto; intros
@@ -449,7 +464,7 @@ Proof.
   eapply exist. intro. unfold decode_next.
   eapply bind_adequate.
   - eapply (take_adequate (Const 1)); constructor.
-  - intros res vres [P0 [P1 P2]].
+  - intros res vres [P0 [P1 P2]]. subst.
     eapply (read_adequate (Var vres) (Const 0)); constructor; auto.
 Defined.
 
@@ -461,7 +476,6 @@ Lemma decode_first_eq : proj1_sig decode_next_DF_example = proj1_sig decode_next
 Fail reflexivity. Abort.
 
 Compute (proj1_sig decode_next_DF).
-
 
 Lemma decode_next_adequate :
   forall data, adequate eq decode_next (`decode_next_DF) data.
@@ -502,7 +516,8 @@ Definition RpacketSSH (s : packet_SSH) (v : (N * N) * (span * span)) :=
 Definition decode_packet_SSH_sig :
   { code | forall data, adequate RpacketSSH decode_packet_SSH code data}.
 Proof.
-  StartDF. repeat FMU32. repeat clean_up. subst.
+  StartDF. repeat FMU32. repeat clean_up.
+  eapply bind_adequate. step. intros. clean_up.
   eapply (ret_adequate _ (Pair (Pair (Var vres) (Var vres0)) (Pair (Var vres1) (Var vres3)))).
   repeat econstructor.
   repeat split; eauto.
